WIP

Tutorial/SPI.v
@@ -1,31 +1,105 @@
 Require Import Coq.Lists.List. Import ListNotations.
-Module spec.
   
-  Axiom one : forall {T}, (T -> Prop) -> list T -> Prop.
-  Axiom plus : forall {T}, (list T -> Prop) -> list T -> Prop.
-  Axiom app : forall {T}, (list T -> Prop) -> (list T -> Prop) -> list T -> Prop.
-  Local Notation "x ^+" := (plus x) (at level 50).
-  Local Infix "+++" := app (at level 60).
-  
+Axiom one : forall {T}, (T -> Prop) -> list T -> Prop.
+Axiom kleene : forall {T}, (list T -> Prop) -> list T -> Prop.
+Axiom plus : forall {T}, (list T -> Prop) -> list T -> Prop.
+Axiom app : forall {T}, (list T -> Prop) -> (list T -> Prop) -> list T -> Prop.
+Axiom either : forall {T}, (list T -> Prop) -> (list T -> Prop) -> list T -> Prop.
+Axiom maybe : forall {T}, (list T -> Prop) -> list T -> Prop.
+Local Notation "x ^*" := (kleene x) (at level 50).
+Local Notation "x ^+" := (plus x) (at level 50).
+Local Infix "+++" := app (at level 60).
+
+Module List. Section __.
+  Context {T : Type}.
+    (* Module interleave.
+    Inductive interleave : list T -> list T -> list T -> Prop :=
+    | nil                                      : interleave     nil    nil    nil
+    | left  x xs ys zs (_:interleave xs ys zs) : interleave (cons x xs) ys (cons x zs)
+    | right y xs ys zs (_:interleave xs ys zs) : interleave (cons y xs) ys (cons y zs).
+    End interleave.
+  Notation interleave := interleave.interleave. *)
+
+  (*
+  Definition interleave_body interleave (zs xs ys : list T) : Prop :=
+    match xs,ys with
+    | [],_ => ys = zs
+    | _,[] => xs = zs
+    | x::xs,y::ys =>
+        match zs with
+        | [] => False
+        | cons z zs => (z = x /\ interleave zs xs ys) \/ (z = y /\ interleave zs xs ys)
+        end
+    end. 
+  *)
+
+  Definition interleave_body interleave (zs xs ys : list T) : Prop :=
+    match zs with
+    | nil => xs = nil /\ zs = nil
+    | cons z zs' =>
+        (exists xs', xs = cons z xs' /\ interleave zs' xs' ys ) \/
+        (exists ys', ys = cons z ys' /\ interleave zs' xs  ys')
+    end.
+  Definition interleave (xs ys zs : list T) : Prop :=
+    (fix interleave zs := interleave_body interleave zs) zs xs ys.
+
+  Lemma interleave_rcons z zs xs ys y (H : z = y) (HH : interleave xs ys zs) : interleave xs (y::ys) (z::zs).
+  Proof. subst; cbn; eauto. Qed.
+  Lemma interleave_lcons z zs xs ys x (H : z = x) (HH : interleave xs ys zs) : interleave (x::xs) ys (z::zs).
+  Proof. subst; cbn; eauto. Qed.
+
+  Lemma interleave_rapp z zs xs ys y (H : z = y) (HH : interleave xs ys zs) : interleave xs (y++ys) (z++zs).
+  Proof. subst; induction y; cbn; eauto. Qed.
+  Lemma interleave_lapp z zs xs ys x (H : z = x) (HH : interleave xs ys zs) : interleave (x++xs) ys (z++zs).
+  Proof. subst; induction x; cbn; eauto. Qed.
+
+  Lemma interleave_nil_r zs : interleave zs nil zs.
+  Proof. induction zs; cbn; eauto. Qed.
+  Lemma interleave_nil_l zs : interleave zs nil zs.
+  Proof. induction zs; cbn; eauto. Qed.
+End __. End List.
+
+
+Module TracePredicate.
   Definition flat_map {A B} (P:A->list B->Prop) xs :=
     List.fold_right app (eq nil) (List.map P xs).
+
+  (* [interleave] trace of *arbitrarily small slices of* [P] and [Q].
+     This sometimes makes sense for completely independent streams of
+     events, but consider [(P \/ Q)^*] instead first. *)
+  Definition interleave {T} (P Q : list T -> Prop) :=
+    fun zs => exists xs ys, List.interleave xs ys zs /\ P xs /\ Q ys.
+
+  Lemma interleave_rapp {T} {P Q : list T -> Prop} z zs
+    (H : Q^* z) (HH : interleave P (Q^* ) zs) : interleave P (Q^* ) (z++zs).
+  Proof.
+    destruct HH as (?&?&?&?&?).
+    eexists _, _; split.
+    eapply List.interleave_rapp; eauto.
+    split; eauto.
+  Admitted.
+  
+  Lemma interleave_lapp {T} {P Q : list T -> Prop} z zs
+    (H : P^* z) (HH : interleave (P^* ) Q zs) : interleave (P^* ) Q (z++zs).
+  Proof.
+    destruct HH as (?&?&?&?&?).
+    eexists _, _; split.
+    eapply List.interleave_lapp; eauto.
+    split; eauto.
+  Admitted.
+
+  Definition interleave_rcons {T} {P Q} (z:T) zs H HH : interleave _ _ (cons _ _) :=
+    @interleave_rapp T P Q [z] zs H HH.
+  Definition interleave_lcons {T} {P Q} (z:T) zs H HH : interleave _ _ (cons _ _):=
+    @interleave_lapp T P Q [z] zs H HH.
   
   Definition at_next_edge {T} clk data : list T -> Prop :=
-    (fun x => not (clk x))^+ +++ (fun x => clk x /\ data x).
-  
-  Definition clk : list (bool * bool * bool) -> Prop :=
-    one (fun '(clk, _, _) => clk = true).
-  Definition mosi : bool -> list (bool * bool * bool) -> Prop :=
-    fun b => one (fun '(_, mosi, _) => mosi = b).
-  Definition miso : bool -> list (bool * bool * bool) -> Prop :=
-    fun b => one (fun '(_, _, miso) => miso = b).
-  
-  (* TODO: allow and ignore nop-s in external io *)
-  Definition mosis := @flat_map bool (bool*bool*bool) (fun x => at_next_edge clk (mosi x)).
-  Definition misos := @flat_map bool (bool*bool*bool) (fun x => at_next_edge clk (miso x)).
-End spec.
+    (fun x => clk false x)^+ +++ (fun x => clk true x /\ data x).
+End TracePredicate.
 
 Require Import Kami.All.
+
+Definition bits {w} : word w -> list bool. Admitted.
 Definition x : nat. exact O. Qed.
 
 Section Named.
@@ -39,7 +113,7 @@ Section Named.
     with Register @^"tx_fifo"     : Bit 8 <- Default
     with Register @^"tx_fifo_len" : Bit 4 <- Default
     with Register @^"rx_fifo"     : Bit 8 <- Default
-    with Register @^"rx_fifo_len" : Bit 4 <- Default
+    with Register @^"rx_fifo_len" : Bit 4 <- @natToWord 4 15
     with Register @^"sck"         : Bool  <- Default
     
     with Rule @^"cycle" := (
@@ -55,19 +129,17 @@ Section Named.
       Call "PutSCK"(#sck : Bool);
       Call "PutMOSI"((UniBit (TruncMsb 7 1) #tx_fifo) : Bit 1);
 
-      If (#tx_fifo_len == $$@natToWord 4 0) then (
-        If (#sck) then (
-          Write @^"tx_fifo" : Bit 8 <- UniBit (TruncLsb 8 1) (BinBit (Concat 8 1) #tx_fifo $$(@ConstBit 1 $x));
-          Write @^"tx_fifo_len" <- #tx_fifo_len - $1;
-          Retv
-        ) else (
-          Write @^"rx_fifo" : Bit 8 <- UniBit (TruncLsb 8 1) (BinBit (Concat 8 1) #rx_fifo #miso);
-          Write @^"rx_fifo_len" : Bit 4 <- #rx_fifo_len + $1;
-          Retv
-        );
-        Retv
-      );
-      Write @^"sck" : Bool <- !#sck;
+      If ((*!*)#tx_fifo_len == $$@natToWord 4 0) then Retv else (If (#sck) then (
+        Write @^"tx_fifo" : Bit 8 <- UniBit (TruncLsb 8 1) (BinBit (Concat 8 1) #tx_fifo $$(@ConstBit 1 $x));
+        Write @^"tx_fifo_len" <- #tx_fifo_len + $1;
+        Write @^"sck" : Bool <- !#sck;
+      Retv ); Retv);
+
+      If (#rx_fifo_len < $$@natToWord 4 8) then (If ((*!*)#sck) then Retv else (
+        Write @^"rx_fifo" : Bit 8 <- UniBit (TruncLsb 8 1) (BinBit (Concat 8 1) #rx_fifo #miso);
+        Write @^"rx_fifo_len" <- #rx_fifo_len - $1;
+        Write @^"sck" : Bool <- !#sck;
+      Retv ); Retv);
 
       Retv
     )
@@ -78,6 +150,7 @@ Section Named.
       If (#tx_fifo_len == $$@natToWord 4 0) then (
         Write @^"tx_fifo" : Bit 8 <- #data;
         Write @^"tx_fifo_len" <- $$@natToWord 4 8;
+        Write @^"rx_fifo_len" <- $$@natToWord 4 0;
         Ret $$false
       ) else (
         Ret $$true
@@ -87,11 +160,12 @@ Section Named.
     
     with Method "read" () : Bool := ( (* TODO return pair *)
       Write @^"hack_for_sequential_semantics" : Bit 0 <- $$(WO);
+      Read rx_fifo_len : Bit 4 <- @^"rx_fifo_len";
       Read rx_fifo <- @^"rx_fifo";
-      Read rx_fifo_len <- @^"rx_fifo_len";
       If (#rx_fifo_len == $$@natToWord 4 8) then (
         LET data : Bit 8 <- #rx_fifo;
         LET err : Bool <- $$false;
+        Write @^"rx_fifo_len" <- $$@natToWord 4 15;
         Ret #err (* TODO: return (data, err) *)
       ) else (
         Ret $$true
@@ -100,91 +174,148 @@ Section Named.
     )
   }.
 
-  Definition iocycle miso sck mosi := eq (Rle (name ++ "_cycle"),
-      [("GetMISO", existT SignT (Void, Bit 1) (wzero 0, miso));
+  Definition cmd_write arg err t := exists r : RegsT, t =
+    [[(r, (Meth ("write", existT SignT (Bit 8, Bool) (arg, err)), @nil MethT))]].
+  Definition cmd_read (ret : word 8) err t := exists r : RegsT, t =
+    [[(r, (Meth ("read", existT SignT (Void, Bool) (wzero 0, err)), @nil MethT))]].
+  Definition iocycle miso sck mosi t := exists r : RegsT, t = [[(r, (Rle (name ++ "_cycle"),
+      [("GetMISO", existT SignT (Void, Bit 1) (wzero 0, WS miso WO));
       ("PutSCK",   existT SignT (Bool, Void)  (sck, wzero 0));
-      ("PutMOSI",  existT SignT (Bit 1, Void) (mosi, wzero 0))]).
-  Definition cmd_write arg err := eq
-    (Meth ("write", existT SignT (Bit 8, Bool) (arg, err)), @nil MethT).
-  Definition cmd_read (ret : word 8) err := eq (* TODO: use "ret" *)
-    (Meth ("read", existT SignT (Void, Bool) (wzero 0, err)), @nil MethT).
+      ("PutMOSI",  existT SignT (Bit 1, Void) (WS mosi WO, wzero 0))]))]].
+  
   Definition nop x := (exists arg, cmd_write arg true x) \/ (exists ret, cmd_read ret true x).
 
-  Definition parsable := Forall (fun l => exists (r:RegsT) x, l = [(r, x)] /\
-    ((exists miso sck mosi, iocycle miso sck mosi x) \/
-     (exists arg err, cmd_write arg err x) \/
-     (exists ret err, cmd_read ret err x))).
+  Definition sck clk t := exists miso mosi, iocycle miso clk mosi t.
+  Definition mosi mosi t := exists sck miso, iocycle miso sck mosi t.
+  Definition miso miso t := exists sck mosi, iocycle miso sck mosi t.
+  
+  (* these are probably not useful because interleaving.. *)
+  Definition mosis := TracePredicate.flat_map (fun x => TracePredicate.at_next_edge sck (mosi x)).
+  Definition misos := TracePredicate.flat_map (fun x => TracePredicate.at_next_edge sck (miso x)).
 
-  Goal forall (I:_->Prop) r l, I r -> Trace SPI r l -> parsable l.
+  Definition exchange tx rx :=
+    cmd_write tx false +++
+    (fun t => mosis (bits tx) t /\ mosis (bits rx) t) +++
+    maybe (cmd_read rx false).
+
+  Definition transaction t := exists tx rx, exchange tx rx t.
+  Definition spec := TracePredicate.interleave nop (kleene (fun t => sck false t \/ transaction t)).
+
+  Definition enforce_regs (regs:RegsT) tx_fifo tx_fifo_len rx_fifo rx_fifo_len sck := regs =
+    [(@^"hack_for_sequential_semantics", existT _ (SyntaxKind (Bit 0)) WO);
+                (@^"tx_fifo", existT _ (SyntaxKind (Bit 8)) tx_fifo);
+                (@^"tx_fifo_len", existT _ (SyntaxKind (Bit 4)) tx_fifo_len);
+                (@^"rx_fifo", existT _ (SyntaxKind (Bit 8)) rx_fifo);
+                (@^"rx_fifo_len", existT _ (SyntaxKind (Bit 4)) rx_fifo_len);
+                (@^"sck", existT _ (SyntaxKind Bool) sck) ].
+
+  (* Local Coercion SyntaxKind : Kind >-> FullKind. *)
+  Record idle (regs : RegsT) (t : list (list FullLabel)) : Prop := {
+    tx_fifo : _ ;
+    rx_fifo : _ ;
+    _ : spec t;
+    _ : enforce_regs regs tx_fifo (natToWord 4 0) rx_fifo (natToWord 4 15) false;
+  }.
+
+  Record active (regs : RegsT) (t : list (list FullLabel)) : Prop := {
+    tx : _;
+    tx_fifo : _ ;
+    tx_fifo_len : _ ;
+    rx_fifo : _ ;
+    rx_fifo_len : _ ;
+    _ : (app spec (cmd_write tx false)) t; (* WIP *)
+    _ : tx = tx_fifo; (* only during first tick *)
+    _ : enforce_regs regs tx_fifo tx_fifo_len rx_fifo rx_fifo_len false;
+  }.
+
+  Definition invariant s t := idle s t \/ active s t.
+
+  Goal forall s t, Trace SPI s t -> invariant s t.
   Proof.
-    intros I r l HI HTrace.
-    induction HTrace.
-    { subst ls'. cbn. admit. }
+    induction 1.
+    { admit. }
+    subst.
+
+    destruct IHTrace as [IHTrace|IHTrace]; [|admit].
+    destruct IHTrace.
+    cbv [enforce_regs] in *.
 
     unshelve (idtac;
     let pf := open_constr:(InvertStep (@Build_BaseModuleWf SPI _) _ _ _ HStep) in
     destruct pf);
     [abstract discharge_wf|..];
     repeat match goal with
+      | H: Trace _ _ |- _ => clear H
       | _ => progress intros
       | _ => progress clean_hyp_step
-      | _ => progress cbn [SPI getMethods baseModule makeModule makeModule' type evalExpr isEq evalConstT Kind_rect app map fst snd projT1 projT2] in *
+      | _ => progress cbn [SPI getMethods baseModule makeModule makeModule' type evalExpr isEq evalConstT Kind_rect List.app map fst snd projT1 projT2] in *
+      | H: UpdRegs _ _ _ |- _ => apply NoDup_UpdRegs in H; symmetry in H; destruct H
     end.
-    15: {
-      erewrite (word0 arg).
-      constructor.
-      2: eapply IHHTrace; admit.
-      eexists ?[r], (?[n], ?[vs]).
-      split; repeat f_equal.
-      right; right.
-      eexists _, _.
-      exact eq_refl. }
 
+    10: {
+      match goal with
+      | H: UpdRegs _ _ _ |- _ => apply NoDup_UpdRegs in H; [symmetry in H; destruct H|..]
+      end.
+      constructor. econstructor.
 
-  Abort.
+      2: cbv [enforce_regs] in *;
+      repeat match goal with
+      | _ => progress discharge_string_dec
+      | _ => progress cbn [fst snd]
+      | |- context G [match ?x with _ => _ end] =>
+         let X := eval hnf in x in
+         progress change x with X
+      | _ => progress (f_equal; [])
+      | |- ?l = ?r =>
+          let l := eval hnf in l in
+          let r := eval hnf in r in
+          progress change (l = r)
+      | _ => exact eq_refl
+      end.
+      2:cbn [evalBinBit evalUniBool].
 
-    (*
-    inversion HStep; subst.
-    inversion HSubsteps; subst.
-    3: {
-      cbn -[SPI] in *.
-      destruct fb as [[argT retT] method].
-      cbn -[SPI] in *.
-      simpl in HInMeths.
+      {
+        cbv [spec].
+        simple refine (TracePredicate.interleave_rcons _ _ _ _).
+        2:eassumption.
+        match goal with |- ?f ?x => enough (sck false x) by admit end.
+        cbv [sck iocycle].
+        eexists _, _, _.
+        repeat f_equal; eauto.
+        1,2: admit. (* bbv... *)
+      }
 
-      clean_hyp_step.
-      clean_hyp_step.
-      assert (sth: Bit 8 = argT). {
-        clear - H1.
-        inversion_sigma.
-        inv H0.
-        auto.
+      idtac.
+      all : cbn [map fst].
+      1,2: admit. (* NoDup *)
     }
-      assert (sth2: Bool = retT). {
-        clear - H1.
-        inversion_sigma.
-        inv H0.
-        auto.
-    }
-      destruct sth, sth2.
-      inversion_sigma.
-      Import Eqdep.
-      Set Printing All.
-      replace (H0) with (eq_refl (Bit 8, Bool)) in H2.
-      2: { symmetry; eapply UIP_refl. }
-      cbn in H2.
-      clear H0.
-      repeat clean_hyp_step.
 
-      Notation "( x , y , .. , z )" := (existT _ .. (existT _ x y) .. z) : core_scope.
 
-      all:
-      try subst method;
-      cbn [type] in *;
-      repeat clean_hyp_step;
-      cbn [evalExpr isEq evalConstT Kind_rect app map fst snd] in *.
+    10: {
+      match goal with
+      | H: UpdRegs _ _ _ |- _ => apply NoDup_UpdRegs in H; [symmetry in H; destruct H|..]
+      end.
+      constructor. econstructor.
 
-      2: {
-        *)
+      2: cbv [enforce_regs] in *;
+      repeat match goal with
+      | _ => progress discharge_string_dec
+      | _ => progress cbn [fst snd]
+      | |- context G [match ?x with _ => _ end] =>
+         let X := eval hnf in x in
+         progress change x with X
+      | _ => progress (f_equal; [])
+      | |- ?l = ?r =>
+          let l := eval hnf in l in
+          let r := eval hnf in r in
+          progress change (l = r)
+      | _ => exact eq_refl
+      end.
+
+
+
+
 
 End Named.
+
+  (* Notation "( x , y , .. , z )" := (existT _ .. (existT _ x y) .. z) : core_scope. *)
